perjit demo proof

theory/JIT.thy
@@ -4,7 +4,7 @@ theory JIT
 imports
   Main
   rBPFCommType rBPFSyntax rBPFSem
-  x64Syntax x64Semantics
+  x64Syntax x64Semantics x64Assembler Proof1
   JIT_def
 begin
 
@@ -95,7 +95,7 @@ fun per_jit_ins ::" bpf_instruction \<Rightarrow> x64_bin option"where
   _ \<Rightarrow> None
 )"
 
-fun jit1 :: "ebpf_asm \<Rightarrow> u8 list \<Rightarrow> usize list \<Rightarrow> (u8 list * usize list) option" where
+(*fun jit1 :: "ebpf_asm \<Rightarrow> u8 list \<Rightarrow> usize list \<Rightarrow> (u8 list * usize list) option" where
 "jit1 [] l_bin l_pc = Some (l_bin, l_pc)" |
 "jit1 (h#t) l_bin l_pc = (
   case per_jit_ins h of
@@ -103,9 +103,9 @@ fun jit1 :: "ebpf_asm \<Rightarrow> u8 list \<Rightarrow> usize list \<Rightarro
   Some ins \<Rightarrow> (
     jit1 t (l_bin @ ins) (l_pc @ [of_nat (length l_bin)])
   )
-)"
+)"*)
 
-fun jit :: "ebpf_asm \<Rightarrow> (u8 list * usize list) option" where
+(*fun jit :: "ebpf_asm \<Rightarrow> (u8 list * usize list) option" where
 "jit [] = Some ([], [])" |
 "jit (h#t) = (
   case jit t of
@@ -116,10 +116,90 @@ fun jit :: "ebpf_asm \<Rightarrow> (u8 list * usize list) option" where
     Some ins \<Rightarrow> Some (ins @l_bin, 0#(map (\<lambda> i. i + (of_nat (length ins))) l_pc))
   )
 )"
+*)
+
+(*
+fun jit :: "ebpf_asm \<Rightarrow> (nat \<times> u64 \<times> x64_bin) list option" where
+"jit [] = Some []" |
+"jit (h#t) = (
+  case jit t of
+  None \<Rightarrow> None |
+  Some l_bin \<Rightarrow> (
+    case per_jit_ins h of
+    None \<Rightarrow> None |
+    Some ins \<Rightarrow> Some ((1,1,ins) #l_bin)
+  )
+)"
+*)
 
 
+fun jit :: "ebpf_asm \<Rightarrow> (nat \<times> u64 \<times> x64_bin) list option" where
+  "jit [] = Some []" |
+  "jit (h#xs) = (case per_jit_ins h of 
+                   None \<Rightarrow> None 
+                 | Some x \<Rightarrow> 
+                     (case jit xs of 
+                        None \<Rightarrow> None 
+                      | Some res \<Rightarrow> Some ((1,1,x) # res)))"
 
+(*
+fun jit :: "ebpf_asm \<Rightarrow> (nat \<times> u64 \<times> x64_bin) list option" where
+"jit [] = Some []" |
+"jit (h#xs) = (case per_jit_ins h of None \<Rightarrow> None | Some x \<Rightarrow> Some ((1,1,x) # the (jit xs)))"
+*)
+
+
+definition jit1 :: "ebpf_asm \<Rightarrow> x64_bin list option" where
+"jit1 ls \<equiv> if \<exists> s \<in> set ls. per_jit_ins s = None then None else 
+  Some ((map the (map per_jit_ins ls)))"
+
+
+(*definition jit :: "ebpf_asm \<Rightarrow> (nat \<times> u64 \<times> x64_bin) list option" where
+"jit ls \<equiv> if \<exists> s \<in> set ls. per_jit_ins s = None then None else 
+  let x = 
+  in Some ((map the (map per_jit_ins ls)))"
+*)
+
+(*definition jit :: "ebpf_asm \<Rightarrow> u8 list list option" where
+"jit ls \<equiv> if \<exists> s \<in> set ls. per_jit_ins s = None then None else Some ((map the (map per_jit_ins ls)))"
+*)                               
+(*
+fun jit :: "ebpf_asm \<Rightarrow> u8 list option" where
+"jit [] = Some []" |
+"jit (h#t) = (
+    case per_jit_ins h of
+    None \<Rightarrow> None |
+    Some ins \<Rightarrow> Some (ins @the (jit t))
+)"
+*)
+
+value "Some ((map the (map per_jit_ins [BPF_ALU64 BPF_ADD BR0 (SOReg BR6),BPF_ALU64 BPF_ADD BR0 (SOReg BR1)])))"
+
+value "jit [BPF_ALU64 BPF_SUB BR0 (SOReg BR6),BPF_EXIT]"
+
+
+(*lemma "\<forall> s \<in> set ls. per_jit_ins s \<noteq> None \<Longrightarrow> jit ls = Some (concat (map the (map per_jit_ins ls)))"
+  apply(cases ls, simp_all)
+  subgoal for a list apply(cases a, simp_all)
+    subgoal for x91 x92 x93 apply(cases x91,simp_all)
+      apply(cases x93, simp_all)
+      subgoal for x2 apply (unfold per_jit_add_reg64_1_def)
+*)
+                 
+value "snd (snd ((the (jit [BPF_EXIT,BPF_EXIT]))!(0::nat)))"
+
+value "jit []"
+
+value "jit [BPF_ALU64 BPF_SUB BR0 (SOReg BR6),BPF_ALU64 BPF_ADD BR0 (SOReg BR6)]"
+
+value "jit [BPF_ALU64 BPF_ADD BR0 (SOReg BR6),BPF_ALU64 BPF_SUB BR0 (SOReg BR6)]"
+
+value "jit [BPF_ALU64 BPF_ADD BR0 (SOReg BR6), BPF_ALU64 BPF_ADD BR0 (SOReg BR6), BPF_EXIT]"
+
+
+value "per_jit_ins (BPF_ALU64 BPF_ADD BR0 (SOReg BR6))"
 (**r simulation relation *)
+(*
 definition match_state :: "sbpf_state \<Rightarrow> x64_state \<Rightarrow> usize list \<Rightarrow> bool" where
 "match_state bst xst pc_map = (
   case bst of
@@ -138,14 +218,33 @@ definition match_state :: "sbpf_state \<Rightarrow> x64_state \<Rightarrow> usiz
   ) |
   _ \<Rightarrow> False
 )"
+*)
+
+definition match_state :: "sbpf_state \<Rightarrow> x64_state \<Rightarrow> bool" where
+"match_state bst xst = (
+  case bst of
+  SBPF_OK pc rs m \<Rightarrow> (
+    case xst of
+      Next xpc xrs xm \<Rightarrow>
+        (\<forall> r. (rs r) = xrs (bpf_to_x64_reg r)) \<and> \<comment>\<open> for ALU + MEM + Call \<close>
+        m = xm  \<comment>\<open> for MEM + Call \<close> |
+      _ \<Rightarrow> False
+  ) |
+  SBPF_Success v \<Rightarrow>(
+    case xst of
+    Next xpc xrs xm \<Rightarrow> v = xrs (bpf_to_x64_reg BR0) \<comment>\<open> for EXIT \<close> |
+      _ \<Rightarrow> False
+  ) |
+  _ \<Rightarrow> False
+)"
 
 lemma x64_sem_add_stuck : 
 " x64_sem (m + n) x64_prog Stuck = xst' \<Longrightarrow>
   x64_sem n x64_prog (x64_sem m x64_prog Stuck) = xst'"
-  apply (cases m; simp)
+  apply (cases m,simp)
   subgoal for m
-    apply (cases n; simp)
-    done
+    apply(cases n,simp)
+    by auto
   done
 
 lemma x64_sem_add: 
@@ -170,20 +269,419 @@ lemma x64_sem_add:
     done
   done
 
-theorem jit_correct:
- "jit prog = Some (x64_prog, pc_map) \<Longrightarrow>
-  bst = SBPF_OK pc rs m \<Longrightarrow>
-  bst' = SBPF_OK pc' rs' m' \<Longrightarrow>
-  xst = Next xpc xrs xm \<Longrightarrow>
-  match_state bst xst pc_map \<Longrightarrow>
-  sbpf_step prog bst = bst' \<Longrightarrow>
-  \<exists> fuel n xst'.
-      x64_sem n x64_prog xst = xst' \<and> \<comment> \<open>
-      x64_sem fuel x64_prog xst' = xst1 \<and> \<close>
-      match_state bst' xst' pc_map"
-  apply simp
-  apply (cases "prog = []"; simp)
+lemma sbpf_sem_induct: 
+  "sbpf_sem (m+n) prog s = s' \<Longrightarrow>
+    \<exists> temps.
+    sbpf_sem m prog s = temps \<and> 
+    sbpf_sem n prog temps = s'"
+  apply (induct m arbitrary: n prog s s')
+  apply simp_all
+  done
 
-  sorry
+lemma sbpf_sem_add: 
+  "sbpf_sem (m+n) prog s = s' \<Longrightarrow>
+    s = (SBPF_OK pc rs mem) \<Longrightarrow>
+    s'\<noteq> SBPF_Err \<Longrightarrow>
+    \<exists> temps.
+    sbpf_sem m prog s = temps \<and> 
+    sbpf_sem n prog temps = s'"
+  using sbpf_sem_induct by blast
+
+lemma sbpf_sem_err: 
+  "sbpf_sem (m+n) prog s = s' \<Longrightarrow>
+    s = SBPF_Err \<Longrightarrow>
+    \<exists> temps.
+    sbpf_sem m prog s = temps \<and> 
+    sbpf_sem n prog temps = s'"
+  using sbpf_sem_induct by blast
+
+lemma err_is_still_err:" sbpf_sem x prog SBPF_Err = s' \<Longrightarrow> s' = SBPF_Err "
+  apply(induct x, simp)
+  by auto
+
+lemma suc_success_is_err:"x > 0 \<Longrightarrow> sbpf_sem x prog (SBPF_Success v) = s' \<Longrightarrow> s' = SBPF_Err "
+  apply(induct x, simp)
+  using err_is_still_err by force
+
+lemma intermediate_step_is_ok:"sbpf_sem x prog s = s' \<Longrightarrow> x > 0 \<Longrightarrow> s' \<noteq> SBPF_Err \<Longrightarrow> \<exists> pc rs mem. s = (SBPF_OK pc rs mem)"
+  apply(induct x arbitrary: prog s s')
+  apply simp 
+  using err_is_still_err suc_success_is_err
+  by (metis sbpf_step.elims)
+
+lemma aluq_subgoal_rr_aux1:
+     "bins = BPF_ALU64 BPF_ADD dst (SOReg src) \<Longrightarrow>
+     xins = Paddq_rr (bpf_to_x64_reg dst) (bpf_to_x64_reg src) \<Longrightarrow>
+     prog!(unat pc) = bins \<Longrightarrow>
+     sbpf_step prog (SBPF_OK pc rs m) = (SBPF_OK pc' rs' m')  \<Longrightarrow>
+     Next spc' reg' m' = exec_instr xins sz spc reg m \<Longrightarrow>
+     reg (bpf_to_x64_reg dst) = rs dst \<Longrightarrow>
+     reg (bpf_to_x64_reg src) = rs src \<Longrightarrow>
+     reg' (bpf_to_x64_reg dst) = (rs' dst)"
+  apply (unfold exec_instr_def step)
+  apply simp
+  apply(cases "prog ! unat pc",simp_all)
+  subgoal for x91 apply(simp split:if_split_asm) 
+    apply(unfold eval_alu_def eval_reg_def,simp_all)
+    by auto
+  done
+
+
+lemma aluq_subgoal_rr_aux2_1:"xins = Paddq_rr dst src \<Longrightarrow> 
+  Next pc' reg' m' = exec_instr xins sz pc reg m \<Longrightarrow>
+  \<forall> r \<noteq> dst. reg' r = reg r"
+  by (simp add: exec_instr_def)
+
+
+lemma aluq_subgoal_rr_aux2:"xins = Paddq_rr (bpf_to_x64_reg dst) (bpf_to_x64_reg src) \<Longrightarrow> 
+  Next pc' reg' m' = exec_instr xins sz pc reg m \<Longrightarrow>
+  \<forall> r \<noteq> dst. reg' (bpf_to_x64_reg r) = reg (bpf_to_x64_reg r)"
+  using aluq_subgoal_rr_aux2_1 by simp
+
+
+lemma aluq_subgoal_rr_aux3:"bins = BPF_ALU64 BPF_ADD dst (SOReg src) \<Longrightarrow> 
+  sbpf_step prog (SBPF_OK pc rs m) = (SBPF_OK pc' rs' m') \<Longrightarrow> 
+  prog!(unat pc) = bins \<Longrightarrow>
+  \<forall> r \<noteq> dst. rs' r = rs r"
+  apply(cases bins,simp_all)
+  apply(cases "prog ! unat pc", simp_all)
+  subgoal for x91 apply(simp split:if_split_asm) 
+    apply(unfold eval_alu_def eval_reg_def,simp_all)
+    by auto
+  done
+
+
+lemma addq_subgoal_rr_generic:
+  assumes a0:"bins = BPF_ALU64 BPF_ADD dst (SOReg src)" and
+       a1:"per_jit_add_reg64_1 dst src = Some l_bin" and
+       a3:"x64_decode 0 l_bin = Some (length l_bin, xins)" and
+       a4:"sbpf_step prog (SBPF_OK pc rs m) = (SBPF_OK pc' rs' m')" and
+       a5:"Next spc' reg' m' = exec_instr xins sz spc reg m" and
+       a6:"match_state (SBPF_OK pc rs m) (Next spc reg m) " and
+       a7:"prog!(unat pc) = bins"
+  shows "match_state (SBPF_OK pc' rs' m') (Next spc' reg' m') "
+proof -
+  have b0:"xins = Paddq_rr (bpf_to_x64_reg dst) (bpf_to_x64_reg src)" using x64_encode_decode_consistency per_jit_add_reg64_1_def a1 a3 
+    by (metis option.inject prod.inject unat_eq_zero)
+    moreover have b1:"(\<forall> r. (rs r) = reg (bpf_to_x64_reg r))" using a6 spec match_state_def by simp
+    moreover have b2:"(rs src) = reg (bpf_to_x64_reg src)" using a6 spec b1 by simp
+    hence b3:"(rs' dst) = reg' (bpf_to_x64_reg dst)" using aluq_subgoal_rr_aux1 b0 b1 b2 a0 a4 a5 a7 by metis
+    have b4:"\<forall> r \<noteq> dst. reg'(bpf_to_x64_reg r) = reg (bpf_to_x64_reg r)" using b0 a5 aluq_subgoal_rr_aux2 by blast
+    have b5:"\<forall> r \<noteq> dst. (rs' r) = (rs r)" using aluq_subgoal_rr_aux3 a0 a4 a7 by force
+    have b6:"\<forall> r \<noteq> dst. (rs r) = reg ((bpf_to_x64_reg r))" using a6 using b1 by blast
+    have b7:"(\<forall> r \<noteq> dst. (rs' r) = reg' ((bpf_to_x64_reg r)))" using b1 b4 b5 by presburger
+    thus ?thesis using b3 match_state_def by force
+  qed
+
+
+lemma exit_subgoal_rr_generic:
+  assumes a0:"bins = BPF_EXIT" and
+       a1:"per_jit_exit = Some l_bin" and
+       a3:"x64_decode 0 l_bin = Some (length l_bin, xins)" and
+       a4:"sbpf_step prog (SBPF_OK pc rs m) = st'" and
+       a5:"xst' = exec_instr xins sz spc reg m" and
+       a6:"match_state (SBPF_OK pc rs m) (Next spc reg m) " and
+       a7:"prog!(unat pc) = bins" and
+       a8:"prog \<noteq> [] \<and> unat pc < length prog \<and> unat pc \<ge> 0"
+     shows "match_state st' xst'"
+proof-
+  have b0:"st' = SBPF_Success (rs BR0)" using a0 a4 a7 a8 by simp
+  have b1:"xins = Pret" using x64_encode_decode_consistency per_jit_exit_def a0 a1 a3
+    by (metis Pair_inject option.inject unat_0)
+  moreover have b2:"(\<forall> r. (rs r) = reg (bpf_to_x64_reg r))" using a6 spec match_state_def by simp
+  moreover have b3:"(rs BR0) = reg (bpf_to_x64_reg BR0)" using a6 spec b2 by simp
+  have b4:"Mem.loadv M64 m ((reg SP) + (u64_of_memory_chunk M64)) \<noteq> None" sorry
+  hence "\<exists> x. Mem.loadv M64 m ((reg SP) + (u64_of_memory_chunk M64)) = x \<and> x\<noteq> None" by simp
+  hence "\<exists> v. Mem.loadv M64 m ((reg SP) + (u64_of_memory_chunk M64)) = Some v" by simp
+  hence b5_1:"\<exists> v. Mem.loadv M64 m ((reg SP) + (u64_of_memory_chunk M64)) = Some (Vlong v)" sorry
+  obtain v where b5_2:"Mem.loadv M64 m ((reg SP) + (u64_of_memory_chunk M64)) = Some (Vlong v)" using b5_1 by blast
+  let "?reg'" = "(reg#SP <- ((reg SP) + (u64_of_memory_chunk M64)))"
+  have b5_3:"\<exists> reg'. xst' = Next v ?reg' m" using exec_instr_def exec_ret_def a5 b1 b5_2 by simp
+  hence b5:"?reg' (bpf_to_x64_reg BR0) = reg (bpf_to_x64_reg BR0)" by (simp add: bpf_to_x64_reg_def)
+  thus ?thesis using exec_instr_def b3 b1 b0 a5 using b5_2 exec_ret_def match_state_def by force
+qed
+
+lemma aux1:"length prog \<noteq> 0 \<and> unat pc < length prog \<and> unat pc \<ge> 0 \<Longrightarrow> 
+  s' = sbpf_step prog s \<Longrightarrow>
+  s = (SBPF_OK pc rs m) \<Longrightarrow> 
+  s' = (SBPF_OK pc' rs' m) \<Longrightarrow> 
+  \<exists> dst src. prog!(unat pc) = BPF_ALU64 BPF_ADD dst (SOReg src)"
+  apply(cases "prog!(unat pc)",simp_all)
+  subgoal for x91 x92 x93 
+   apply(unfold eval_alu_def Let_def)
+    apply(cases x91,simp_all) 
+    apply(cases x93, simp_all)
+    done
+  done
+
+lemma aux2:"length prog \<noteq> 0 \<and> unat pc < length prog \<and> unat pc \<ge> 0 \<Longrightarrow> 
+  s' = sbpf_step prog s \<Longrightarrow>
+  s = (SBPF_OK pc rs m) \<Longrightarrow> 
+  s' \<noteq> SBPF_Err \<Longrightarrow> 
+  \<exists> dst src. prog!(unat pc) = BPF_ALU64 BPF_ADD dst (SOReg src) \<or> prog!(unat pc) = BPF_EXIT"
+  apply(cases "prog!(unat pc)",simp_all)
+  subgoal for x91 x92 x93 
+   apply(unfold eval_alu_def Let_def)
+    apply(cases x91,simp_all) 
+    apply(cases x93, simp_all)
+    done
+  done
+
+
+lemma aux3:"jit prog = Some x64_prog \<Longrightarrow> length x64_prog = length prog"
+proof (induction prog arbitrary: x64_prog)
+  case Nil
+  then show ?case by simp
+next
+  case (Cons h xs)
+  assume "jit (h # xs) = Some x64_prog"
+  then have a0:"\<exists> x. per_jit_ins h = Some x" using Cons(1) by (cases "per_jit_ins h"; auto)
+  obtain x where a1:"per_jit_ins h = Some x" using a0 by auto
+  then have a2:"\<exists> res. jit xs = Some res" using Cons(1) apply (cases "jit xs"; auto) 
+    using Cons.prems(1) by force
+  obtain res where a3:"jit xs = Some res" using a2 by auto
+  have a4:"x64_prog = (1, 1, x) # res" using Cons(1) a3 a1
+    using Cons.prems(1) by force
+  then have a5:"length ( x64_prog) = length (h # xs)" using a4 Cons.IH a3 by fastforce
+  then show ?case using Cons by simp
+qed
+
+
+value "[2::nat,3]!(unat (0::u64))"
+
+lemma aux4:"jit prog = Some x64_prog \<Longrightarrow> unat pc \<ge> 0 \<and> unat pc < length prog \<Longrightarrow> 
+  prog!(unat pc) = bins \<Longrightarrow> x64_prog!(unat pc) = l_bin \<Longrightarrow> prog \<noteq> [] 
+  \<Longrightarrow> Some (snd(snd l_bin)) = per_jit_ins bins"
+proof (induction prog arbitrary: x64_prog pc bins l_bin)
+  case Nil
+  then show ?case by simp
+next
+  case (Cons a prog)
+  then show ?case
+  proof-
+    have a0:"unat pc = 0 \<or> unat pc \<ge> 1" by auto
+    show ?thesis
+    proof (cases "unat pc = 0")
+      case True
+      have "unat pc = 0" using True a0 by simp
+      have b0:"\<exists> x. per_jit_ins a = Some x" using Cons by (cases "per_jit_ins a"; auto)
+      obtain x where b1:"per_jit_ins a = Some x" using b0 by auto
+      then have b2:"\<exists> res. jit prog = Some res" using Cons(1) apply (cases "jit prog"; auto) 
+        using Cons.prems(1) by force
+      obtain res where b3:"jit prog = Some res" using b2 by auto
+      have b4:"x64_prog = (1, 1, x) # res" using Cons(1) b3 b1 Cons by force
+      have bn:"Some (snd (snd l_bin)) = per_jit_ins bins" using b1 b2 
+        using Cons.prems(3) Cons.prems(4) True b4 by fastforce
+      then show ?thesis using bn by blast
+    next
+      case False
+      let "?x" = "the (jit prog)"
+      have c0:"\<exists> x. Some ((1, 1, x) # ?x) = Some x64_prog" using Cons 
+        by (metis (no_types, lifting) jit.simps(2) option.case_eq_if option.discI)
+      have c1:"unat pc \<ge> 1" using a0 False by blast
+      have c2:"(a#prog) ! unat pc = bins" using c0 Cons.prems(3) by blast
+      let "?pc'" = "unat pc -1"
+      have c4:"0 \<le> ?pc' \<and> ?pc' < length prog \<and>
+      prog ! ?pc' = bins \<and> ?x ! ?pc' = l_bin \<and> prog \<noteq> []" using Cons.prems(2) Cons.prems(3) Cons.prems(4) c0 c1 by auto
+      (* have cn:"0 \<le> unat pc \<and> unat pc < length prog \<Longrightarrow> 
+  prog ! unat pc = bins \<Longrightarrow> ?x ! unat pc = l_bin \<Longrightarrow> Some (snd (snd l_bin)) = per_jit_ins bins" using Cons
+        by (metis (no_types, lifting) jit.simps(2) option.case_eq_if option.collapse)*)
+      have c5:"Some (snd (snd l_bin)) = per_jit_ins bins" using c4 Cons 
+        by (metis (no_types, lifting) False jit.simps(2) option.case_eq_if option.collapse option.discI order_neq_le_trans unat_gt_0 unat_minus_one)
+      then show ?thesis using c5 by blast
+    qed
+  qed
+qed
+
+
+(*lemma aux3:"jit prog = x64_prog \<Longrightarrow> x64_prog \<noteq> None \<Longrightarrow> length (the x64_prog) = length prog"
+  by (metis length_map option.sel)
+
+lemma aux4:"jit prog = x64_prog \<Longrightarrow> x64_prog \<noteq> None \<Longrightarrow> unat pc \<ge> 0 \<and> unat pc < length prog \<Longrightarrow> prog \<noteq> [] \<Longrightarrow>
+  prog!(unat pc) = bins \<Longrightarrow> (the x64_prog)!(unat pc) = l_bin 
+  \<Longrightarrow> Some l_bin = per_jit_ins bins"
+  using jit_def aux3 by (metis (no_types, lifting) list.map_comp map_equality_iff nth_map nth_mem option.collapse option.sel)
+*)
+
+lemma demo1: assumes a0:"s' = sbpf_step prog s" and
+  a1:"s = (SBPF_OK pc rs m)" and
+  a2:"s' = (SBPF_OK pc' rs' m)" and
+  a3:"xst = (Next xpc xrs m)" and
+  a4:"match_state s xst" and
+  a5:"jit prog = Some x64_prog" and
+  a6:"prog \<noteq> [] \<and> unat pc < length prog \<and> unat pc \<ge> 0" and
+  a7:"xpc = 0" 
+shows "\<exists> xst'. let l = (x64_prog!(unat pc)) in x64_sem 1 (snd (snd l)) xst = xst' \<and> 
+  match_state s' xst'"
+(* \<and> snd xst' = unat (pc+1)*)
+proof-
+  let "?bpf_ins" = "prog!(unat pc)"
+  have b0:"length prog \<noteq> 0" using a6 by blast
+  have b1:"\<exists> src dst. ?bpf_ins = BPF_ALU64 BPF_ADD dst (SOReg src)" using a0 a1 a2 a6 b0 aux1 by blast
+  obtain src dst where b2:"?bpf_ins = BPF_ALU64 BPF_ADD dst (SOReg src)" using b1 by blast
+  let "?l_bin"= "the (per_jit_ins ?bpf_ins)"
+  have c0:"(?l_bin = the (per_jit_add_reg64_1 dst src))" using b2 by fastforce
+  have c1:"Some ?l_bin = x64_encode (Paddq_rr (bpf_to_x64_reg dst) (bpf_to_x64_reg src))" using per_jit_add_reg64_1_def c0 by fastforce
+  have c2:"snd (snd (x64_prog!(unat pc))) = ?l_bin" using a6 c0 a5 aux4 by (metis option.sel)
+  let "?st" = "x64_sem 1 ?l_bin xst"
+  have c3:"\<exists> size2 xins2. x64_decode 0 ?l_bin = Some (length ?l_bin, xins2) \<and> ?st = exec_instr xins2 size2 xpc xrs m" using x64_encode_decode_consistency a3 a7 c1 by fastforce
+  obtain size2 xins2 where c4:"x64_decode 0 ?l_bin = Some (length ?l_bin, xins2) \<and> ?st = exec_instr xins2 size2 xpc xrs m" using c3 by auto
+  have c5:"xins2 = Paddq_rr (bpf_to_x64_reg dst) (bpf_to_x64_reg src)" using Pair_inject c4 c1 option.inject x64_encode_decode_consistency by metis
+  have c6:"\<exists> xrs' xpc'. ?st = Next xpc' xrs' m" using exec_instr_def spec c5 c4 by auto
+  obtain xrs' xpc' where c7:"?st = Next xpc' xrs' m" using c6 by auto
+  have c8:"match_state s' ?st" using addq_subgoal_rr_generic by (metis a0 a1 a2 c7 a4 a3 c1 per_jit_add_reg64_1_def b2 c4)
+    show ?thesis using c8 c2 by simp
+  qed
+
+lemma match_s_not_stuck:"match_state s xst \<Longrightarrow> xst \<noteq> Stuck"
+  apply(cases s, simp_all)
+  apply(unfold match_state_def)
+  subgoal for x11 x12 x13 by auto
+  subgoal for x2 by auto
+  by simp
+
+lemma mem_is_not_changed:"s2 = sbpf_step prog s1 \<Longrightarrow> s1 = (SBPF_OK pc1 rs1 m1) \<Longrightarrow> s2 = (SBPF_OK pc2 rs2 m2) \<Longrightarrow> m1 = m2"
+  apply(cases "prog!(unat pc1)", simp_all)
+  subgoal for x11 x12 x13 
+    by (metis bpf_instruction.simps(361) sbpf_state.simps(6))
+  subgoal for x21 x22 x23 x24
+    by (metis bpf_instruction.simps(362) sbpf_state.simps(6))
+  subgoal for x31 x32 x33 x34 
+    by (metis bpf_instruction.simps(363) sbpf_state.simps(6))
+  subgoal for x4 
+    by (metis bpf_instruction.simps(364) sbpf_state.distinct(3))
+  subgoal for x51 x52 x53 
+    by (metis bpf_instruction.simps(365) sbpf_state.simps(6))
+  subgoal for x6 
+    by (metis bpf_instruction.simps(366) sbpf_state.simps(6))
+  subgoal for x71 x72
+    by (metis bpf_instruction.simps(367) sbpf_state.simps(6))
+  subgoal for x81 x82
+    by (metis bpf_instruction.simps(368) sbpf_state.simps(6))
+  subgoal for x91 x92 x93
+    apply(split if_splits, simp_all)
+    apply(split if_splits, simp_all)
+    apply(cases x91, simp_all)
+    apply(cases "eval_alu BPF_ADD x92 x93 rs1", simp_all)
+    done
+  subgoal for x10
+    by (metis bpf_instruction.simps(370) sbpf_state.simps(6))
+  subgoal for x111 x112
+    by (metis bpf_instruction.simps(371) sbpf_state.simps(6))
+  subgoal for x121 x122 x123
+    by (metis bpf_instruction.simps(372) sbpf_state.simps(6))
+  subgoal for x131 x132 x133
+    by (metis bpf_instruction.simps(373) sbpf_state.simps(6))
+  subgoal for x141 x142 x143
+    by (metis bpf_instruction.simps(374) sbpf_state.simps(6))
+  subgoal for x15
+    by (metis bpf_instruction.simps(375) sbpf_state.simps(6))
+  subgoal for x161 x162 x163 x164
+    by (metis bpf_instruction.simps(376) sbpf_state.simps(6))
+  subgoal for x171 x172
+    by (metis bpf_instruction.simps(377) sbpf_state.simps(6))
+  subgoal for x181 x182
+    by (metis bpf_instruction.simps(378) sbpf_state.simps(6))
+  by (metis (no_types, lifting) bpf_instruction.simps(379) sbpf_state.distinct(1) sbpf_state.simps(6))             
+
+lemma mem_is_not_changed2:"x64_sem 1 l xst1 = xst2 \<Longrightarrow> xst1 = Next xpc1 xrs1 m1 \<Longrightarrow> xst2 = Next xpc2 xrs2 m2 \<Longrightarrow> m1 = m2"
+  apply(cases "x64_decode (unat xpc1) l", simp_all)
+  subgoal for a apply(cases a, simp_all)
+    subgoal for aa b
+      apply(unfold exec_instr_def)
+      apply (cases b, simp_all)
+      apply(unfold exec_ret_def Let_def) 
+      apply(cases "loadv M64 m1 (xrs1 SP + u64_of_memory_chunk M64)", simp_all)
+      subgoal for ab apply(cases ab, simp_all)
+        done
+      done
+    done
+  done
+
+lemma x64_sem1_induct:"x64_sem1 (Suc n) pc x64_prog xst = xst' \<Longrightarrow>
+  xst1 = Next xpc1 xrs1 m \<Longrightarrow> xpc1 = 0 \<Longrightarrow> x64_sem1 n pc x64_prog xst = xst1 \<Longrightarrow> 
+  x64_sem 1 (snd (snd ((x64_prog!(unat pc'))))) xst1 = xst'"
+ apply(induct n arbitrary:pc x64_prog xst xst' xst1 xpc1 xrs1 m pc')
+   apply simp
+  apply(cases "x64_decode 0 (snd (snd (x64_prog ! unat pc')))", simp_all)
+  subgoal for pc x64_proga xst xst' xst1 xpc1 xrs1 m pc'
+    apply(cases "x64_proga ! unat pc", simp_all)
+    subgoal for a b c apply(cases "x64_decode 0 (snd (snd (x64_proga ! unat pc')))",simp_all)
+      sorry
+    done
+  subgoal for pc x64_proga xst xst' xst1 xpc1 xrs1 m a pc'
+    apply(cases "x64_proga ! unat pc", simp_all)
+    subgoal for aa b c apply(cases "x64_decode 0 (snd (snd (x64_proga ! unat a)))", simp_all) sorry
+    done
+  subgoal for n pc x64_prog xst xst' xst1 xpc1 xrs1 m pc' apply(cases "x64_prog ! unat pc", simp_all)
+    done
+  done
+
+lemma demo2:
+  "\<lbrakk> sbpf_sem n prog s = s';
+   s = (SBPF_OK pc rs m);
+   s' = (SBPF_OK pc' rs' m);
+   xst = (Next xpc xrs m);
+   match_state s xst;
+   jit prog = Some x64_prog;
+   prog \<noteq> [] \<and> unat pc < length prog \<and> unat pc \<ge> 0;
+   xpc = 0;
+   x64_sem1 n pc x64_prog xst = xst' \<rbrakk> \<Longrightarrow>
+   match_state s' xst'"
+(* \<exists> xst'. x64_sem1 n pc x64_prog xst = xst' \<and> match_state s' xst'"*)
+proof (induction n arbitrary: prog s s' pc rs m pc' rs' xst' xst xpc xrs x64_prog xst')
+  case 0
+  then show ?case
+    by simp
+next
+  case (Suc n)
+  assume assm1: "sbpf_sem (Suc n) prog s = s'" and
+       assm2:"s = SBPF_OK pc rs m" and
+       assm3:"s' = SBPF_OK pc' rs' m" and
+       assm4:"xst = Next xpc xrs m" and
+       assm5:"match_state s xst" and
+       assm6:"jit prog = Some x64_prog" and
+       assm7:"prog \<noteq> [] \<and> unat pc < length prog \<and> 0 \<le> unat pc " and
+       assm8:"xpc = 0" and
+       assm9:"x64_sem1 (Suc n) pc x64_prog xst = xst'"
+  then obtain s1 where s1_eq: "s' = sbpf_step prog s1" 
+    by (metis add_Suc_right sbpf_sem.simps(1) sbpf_sem.simps(2) sbpf_sem_induct)
+  from Suc have s'_def:"sbpf_sem (Suc n) prog s = s'" by blast
+  have one_step_def:"\<exists> s1. sbpf_sem n prog s = s1 \<and> sbpf_step prog s1 = s'" using s1_eq s'_def sbpf_sem_induct
+    by (metis add_Suc_right sbpf_sem.simps(1) sbpf_sem.simps(2))
+  obtain s1 where get_s1:"sbpf_sem n prog s = s1 \<and> sbpf_step prog s1 = s'" using one_step_def by simp
+  have a1:"s1 = sbpf_sem n prog s" using one_step_def s1_eq using get_s1 by force
+  have a3:"\<exists> pc1 rs1 m1. s1 = (SBPF_OK pc1 rs1 m1)" 
+    by (smt (verit) Suc.prems(3) get_s1 sbpf_state.simps(6) sbpf_step.elims)
+  obtain pc1 rs1 m1 where "s1 = (SBPF_OK pc1 rs1 m1)" using a3 by auto
+  moreover have "m1 = m" using mem_is_not_changed Suc.prems(3) calculation get_s1 by blast
+  hence a4:"s1 = (SBPF_OK pc1 rs1 m)" using calculation by blast
+  have "\<exists> xst1. x64_sem1 n pc x64_prog xst = xst1" by blast
+  (*have "\<exists> xst1. x64_sem1 n pc x64_prog xst = xst1 \<and> x64_sem 1 (snd (snd ((x64_prog!(unat pc1))))) xst1 = xst'" sorry*)
+  then obtain xst1 where a2:"x64_sem1 n pc x64_prog xst = xst1" using a4 by auto
+  from Suc.IH have "sbpf_sem n prog s = s' \<Longrightarrow>
+           s = SBPF_OK pc rs m \<Longrightarrow>
+           s' = SBPF_OK pc' rs' m \<Longrightarrow>
+           xst = Next xpc xrs m \<Longrightarrow>
+           match_state s xst \<Longrightarrow>
+           jit prog = Some x64_prog \<Longrightarrow>
+           prog \<noteq> [] \<and> unat pc < length prog \<and> 0 \<le> unat pc \<Longrightarrow> xpc = 0 \<Longrightarrow> x64_sem1 n pc x64_prog xst = xst' \<Longrightarrow> 
+           match_state s' xst'" by blast
+  from Suc have a5:"match_state s1 xst1" using a1 assm2 a4 assm4 assm5 assm6 assm7 assm8 a2 by blast
+  have b0:"\<exists> xpc1 xrs1 m2. xst1 = (Next xpc1 xrs1 m2)" using match_s_not_stuck a5 by (meson outcome.exhaust)
+  obtain xpc1 xrs1 m2 where "xst1 = (Next xpc1 xrs1 m2)" using b0 by auto
+  moreover have "m2 = m" using a4 a5 calculation(2) match_state_def by auto
+  hence b2:"xst1 = (Next xpc1 xrs1 m)" using calculation by blast
+  have b3:"xpc1 = 0" sorry
+  have b4:"unat pc1 < length prog \<and> unat pc1 \<ge> 0" 
+    by (metis (no_types, lifting) a4 assm3 get_s1 linorder_not_less sbpf_state.simps(6) sbpf_step.simps(1))
+  have b6:"\<exists> xst2. x64_sem 1 (snd (snd ((x64_prog!(unat pc1))))) xst1 = xst2 \<and> match_state s' xst2" 
+    using s1_eq a4 assm3 b2 a5 assm6 assm7 b3 demo1 b4 by (metis get_s1)
+  obtain xst2 where "x64_sem 1 (snd (snd ((x64_prog!(unat pc1))))) xst1 = xst2 \<and> match_state s' xst2" using b6 by auto
+  moreover have "xst2 = xst'" using x64_sem1_induct 
+    using a2 assm9 b3 calculation(2) calculation(3) by blast
+  then show ?case  using calculation(3) by fastforce
+qed
+
 
 end
