theory/x64Semantics.thy
@@ -3,10 +3,10 @@ section \<open> x64 Semantics \<close>
 theory x64Semantics
 imports
   Main
-  rBPFCommType Val Mem x64Syntax
+  rBPFCommType Val Mem x64Syntax x64Disassembler
 begin
 
-axiomatization x64_decode :: "nat \<Rightarrow> u8 list \<Rightarrow> (nat * instruction) option"
+(*axiomatization x64_decode :: "nat \<Rightarrow> u8 list \<Rightarrow> (nat * instruction) option"*)
 
 text \<open> define our x64 semantics in Isabelle/HOL, following the style of CompCert x64 semantics: https://github.com/AbsInt/CompCert/blob/master/x86/Asm.v  \<close>
 
@@ -45,6 +45,17 @@ definition exec_instr :: "instruction \<Rightarrow> u64 \<Rightarrow> u64 \<Righ
   _               \<Rightarrow> Stuck
 )"
 
+(*fun x64_sem :: "nat \<Rightarrow> x64_bin \<Rightarrow> outcome \<Rightarrow> outcome" where
+"x64_sem 0 _ st = st" |
+"x64_sem _ _ Stuck = Stuck" |
+"x64_sem (Suc n) l (Next pc rs m) = (
+  case x64_decode (unat pc) l of
+  None \<Rightarrow> Stuck |
+  Some (sz, ins) \<Rightarrow>
+    x64_sem n l (exec_instr ins (of_nat sz) pc rs m)
+)"
+*)
+
 fun x64_sem :: "nat \<Rightarrow> x64_bin \<Rightarrow> outcome \<Rightarrow> outcome" where
 "x64_sem 0 _ st = st" |
 "x64_sem _ _ Stuck = Stuck" |
@@ -54,6 +65,63 @@ fun x64_sem :: "nat \<Rightarrow> x64_bin \<Rightarrow> outcome \<Rightarrow> ou
   Some (sz, ins) \<Rightarrow>
     x64_sem n l (exec_instr ins (of_nat sz) pc rs m)
 )"
+
+fun x64_sem1 :: "nat \<Rightarrow> u64 \<Rightarrow> (nat \<times> u64 \<times> x64_bin) list \<Rightarrow> outcome \<Rightarrow> outcome" where
+"x64_sem1 0 _ _ st = st" |
+"x64_sem1 (Suc n) pc lt xst = (let (num,off,l) = lt!(unat pc) in
+                       let xst_temp = (case xst of (Next xpc rs m) \<Rightarrow> Next 0 rs m | Stuck \<Rightarrow> Stuck) in
+                       let xst' = x64_sem num l xst_temp in (x64_sem1 n (pc+off) lt xst'))"
+
+
+(*definition x64_sem1 ::"nat \<Rightarrow> (nat \<times> x64_bin) list \<Rightarrow> outcome \<Rightarrow> outcome" where
+"x64_sem1 pc lt xst \<equiv> (let (fuel,l) = lt!pc in
+                       let xst_temp = (case xst of (Next xpc rs m) \<Rightarrow> Next 0 rs m | Stuck \<Rightarrow> Stuck) in
+                       let xst' = x64_sem fuel l xst_temp in (xst', pc+1))"*)
+
+value "length [1::nat,2,3]"
+
+(*fun x64_sem1 ::"nat \<Rightarrow> x64_bin \<Rightarrow> outcome \<Rightarrow> (outcome \<times> nat)" where
+"x64_sem1 pc l Stuck = (Stuck, pc)" |
+"x64_sem1 pc l (Next pc rs m) = (case x64_decode (unat pc) l of
+  None \<Rightarrow> Stuck |
+  Some (sz, ins) \<Rightarrow>
+    x64_sem1 n l (exec_instr ins (of_nat sz) pc rs m))"
+*)
+(*
+fun interp3 :: "instruction list \<Rightarrow> outcome \<Rightarrow> outcome" where
+"interp3 [] s = s" |
+"interp3 (ins#l) st = (
+  case st of
+  Stuck \<Rightarrow> Stuck |
+  Next rs m \<Rightarrow> (
+        interp3 l (exec_instr ins 1 rs m)
+))"
+*)
+
+definition init_reg_map :: "regset" where
+"init_reg_map = (\<lambda> _. 0) (RAX:= 0b00000011, RBX:= 0b00000001)"
+
+definition init_map::"mem" where
+"init_map = Map.empty"
+
+value "init_reg_map RBX"
+
+value "init_reg_map RCX"
+
+value "init_mem 0"
+
+value "x64_sem 2 [0b01001000,0b00000001,0b11011000,0b11000011] (Next (0::u64) (init_reg_map) m)"
+value "x64_sem 1 [0b01001000,0b00000001,0b11011000,0b11000011] (Next (0::u64) (init_reg_map) m)"
+value "x64_sem 0 [0b01001000,0b00000001,0b11011000,0b11000011] (Next (0::u64) (init_reg_map) m)"
+
+value "x64_sem 1 [0b11000011] (Next (0::u64) (init_reg_map) m)"
+
+value "x64_sem 2 [0b11000011] (Next (0::u64) (init_reg_map) m)"
+
+value "x64_sem1 (2::nat) 1 [((1::nat),(1::u64),[0b01001000,0b00000001,0b11011000]),((1::nat),(1::u64),[0b11000011])] (Next (0::u64) (init_reg_map) m)"
+
+lemma "x64_sem1 (1::nat) 1 [((1::nat),(1::u64),[0b01001000,0b00000001,0b11011000]),((1::nat),(1::u64),[0b11000011])] (Next xpc rs m)  = exec_instr Pret 1 0 rs m "
+  using x64_decode_def by simp
 
 type_synonym x64_state = outcome
 
