theory/Proof1.thy
@@ -1,0 +1,21 @@
+theory Proof1
+imports
+  Main
+  rBPFCommType rBPFSyntax x64Assembler x64Disassembler
+
+begin
+
+value "x64_decode 0 (the (x64_encode (Paddq_rr RAX RBX)))"
+           
+lemma x64_encode_decode_consistency:
+  "Some l_bin = x64_encode ins \<Longrightarrow>
+    x64_decode 0 l_bin = Some (length l_bin, ins)"
+  apply(cases ins,simp_all)
+   prefer 2 apply(unfold x64_decode_def, simp_all)
+  subgoal for dst src 
+        apply (unfold Let_def construct_rex_to_u8_def construct_modsib_to_u8_def)
+    subgoal by (cases src; simp;cases dst; auto simp add: x64_decode_def bitfield_insert_u8_def Let_def ireg_of_u8_def
+          Suc3_eq_add_3 add.commute)
+    done
+  done
+end
